Progress.v
@@ -1,85 +1,75 @@
 From SFL Require Import Imports Terms Auxiliaries Typecheck Eval.
 Require Import Coq.Strings.String.
 
-Lemma progressPre: forall t,
-  istypechecked nil t  = true ->
-  (isvalue t = true) \/ (exists t', term_eqbO (beta t) (Some t') = true).
-Proof. intros t Htc.
-       induction t; intros.
+
+Lemma progress: forall t T,
+  typecheck nil t  = Some T ->
+  (isvalue t = true) \/ (exists t', beta t = Some t').
+Proof. intros t.
+       induction t; intros T Htc.
        - right. cbn in *. easy.
        - cbn. now left.
        - right.
+         apply istypechecked_app in Htc.
+         destruct Htc as (U, (Ha, Hb)).
          specialize (isvalue_dec t1); intros it1.
-         destruct it1 as [it1 | it1].
+         destruct it1 as [it1 | it1]. 
          + specialize (isvalue_dec t2) as [it2 | it2].
            ++ case_eq t1.
               * intros x Ht1. subst. easy.
               * intros x tx e.
                 cbn. rewrite it2. exists (subst e x t2).
-                now rewrite term_eqbO_refl.
+                easy.
               * intros. subst. cbn in *. easy.
-              * intros n Ht1. rewrite Ht1 in Htc.
-                contradict Htc; easy.
-              * intros n Ht1. rewrite Ht1 in Htc.
-                contradict Htc; easy.
-              * intros. subst. cbn in *. easy.
-              * intros. subst. cbn in *. easy.
+              * intros n Ht1. rewrite Ht1 in Ha.
+                contradict Ha; easy.
+              * intros n Ht1. rewrite Ht1 in Ha.
+                contradict Ha; easy.
               * intros. subst. cbn in *. easy.
               * intros. subst. cbn in *. easy.
               * intros. subst. cbn in *. easy.
               * intros. subst. cbn in *. easy.
               * intros. subst. cbn in *. easy.
-           ++ assert (Htt2: istypechecked nil t2 = true).
-              { apply istypechecked_t2 in Htc. easy. }
-              specialize (IHt2 Htt2).
+              * intros. subst. cbn in *. easy.
+              * intros. subst. cbn in *. easy.
+           ++ specialize (IHt2 _ Hb).
               destruct IHt2 as [it2' | Hstep].
               +++ rewrite it2 in it2'. easy.
               +++ destruct Hstep as (t2', Hstep).
                   case_eq t1.
                   * intros. subst. easy.
                   * cbn. intros x tx e Ht1. rewrite it2.
-                    apply term_eqbO_eq in Hstep.
                     rewrite Hstep.
-                    exists (App (Lambda x tx e) t2').
-                    now rewrite term_eqbO_refl.
+                    exists (App (Lambda x tx e) t2'). easy.
                  * intros. subst. cbn in *. easy.
-                 * intros n Ht1. rewrite Ht1 in Htc.
-                   contradict Htc; easy.
-                 * intros b Ht1. rewrite Ht1 in Htc.
-                   contradict Htc; easy.
-                 * intros. subst. cbn in *. easy.
+                 * intros n Ht1. rewrite Ht1 in Ha.
+                   contradict Ha; easy.
+                 * intros b Ht1. rewrite Ht1 in Ha.
+                   contradict Ha; easy.
                  * intros. subst. cbn in *. easy.
                  * intros. subst. cbn in *. easy.
                  * intros. subst. cbn in *. easy.
                  * intros. subst. cbn in *. easy.
                  * intros. subst. cbn in *. easy.
                  * intros. subst. cbn in *. easy.
-         + assert (Htt1: istypechecked nil t1 = true).
-           { apply istypechecked_t1 in Htc. easy. }
-           specialize (IHt1 Htt1).
+                 * intros. subst. cbn in *. easy.
+         + specialize (IHt1 _ Ha).
            destruct IHt1 as [IHt1 | IHt1].
            ++ rewrite it1 in IHt1. contradict IHt1; easy.
            ++ destruct IHt1 as (t1', Hstep). cbn.
               rewrite it1. 
-              apply term_eqbO_eq in Hstep.
               rewrite Hstep.
-              case_eq t1; try (intros; exists (App t1' t2); rewrite term_eqbO_refl; easy).
+              case_eq t1; try (intros; exists (App t1' t2); easy).
               intros x tx e Ht1.
               rewrite Ht1 in it1. easy.
        - cbn. now left.
        - cbn. now left.
        - right.
-         unfold istypechecked in Htc.
-         case_eq (typecheck nil (ITE t1 t2 t3)). intros t Htca.
-         apply istypechecked_ite2 in Htca.
-         destruct Htca as (Ha, (Hb, Hc)).
-         unfold istypechecked in IHt1, IHt2, IHt3.
-         rewrite Ha in IHt1.
-         rewrite Hb in IHt2.
-         rewrite Hc in IHt3.
-         specialize (IHt1 eq_refl).
-         specialize (IHt2 eq_refl).
-         specialize (IHt3 eq_refl).
+         apply istypechecked_ite in Htc.
+         destruct Htc as (Ha, (Hb, Hc)).
+         specialize (IHt1 _ Ha).
+         specialize (IHt2 _ Hb).
+         specialize (IHt3 _ Hc).
          destruct IHt1 as [t1'| Hstep].
          + case_eq t1.
            ++ intros. subst. easy.
@@ -90,8 +80,8 @@ Proof. intros t Htc.
            ++ intros. rewrite H in Ha. contradict Ha; easy.
            ++ intros. cbn. 
               case_eq b; intros.
-               * exists t2. rewrite term_eqbO_refl. easy.
-               * exists t3. rewrite term_eqbO_refl. easy.
+               * exists t2. easy.
+               * exists t3. easy.
            ++ intros. subst. cbn in *. easy.
            ++ intros. subst. cbn in *. easy.
            ++ intros. subst. cbn in *. easy.
@@ -100,14 +90,12 @@ Proof. intros t Htc.
            ++ intros. subst. cbn in *. easy.
            ++ intros. subst. cbn in *. easy.
          + destruct Hstep as (t1', Hstep).
-           apply term_eqbO_eq in Hstep. cbn.
+           cbn.
            rewrite Hstep.
-           case_eq t1; intros; try (exists (ITE t1' t2 t3); rewrite term_eqbO_refl; easy).
+           case_eq t1; intros; try (exists (ITE t1' t2 t3); easy).
            rewrite H in Hstep. easy.
-         + intros. rewrite H in Htc. easy.
-       - pose proof Htc as Htc0.
-         apply istypechecked_st in Htc.
-         specialize (IHt Htc).
+       - apply istypechecked_fix in Htc.
+         specialize (IHt _ Htc).
          destruct IHt as [ IHt | IHt ].
          + cbn. right.
            pose proof IHt as HH.
@@ -116,13 +104,12 @@ Proof. intros t Htc.
            case_eq t.
            ++ intros. subst. easy.
            ++ intros x tx e Ht.
-              exists (subst e x (Fix (Lambda x tx e))).
-              rewrite term_eqbO_refl. easy.
+              exists (subst e x (Fix (Lambda x tx e))). easy.
            ++ intros. subst. easy.
-           ++ intros n Ht; rewrite Ht in Htc0;
-              contradict Htc0; easy.
-           ++ intros b Ht; rewrite Ht in Htc0;
-              contradict Htc0; easy.
+           ++ intros n Ht; rewrite Ht in Htc;
+              contradict Htc; easy.
+           ++ intros b Ht; rewrite Ht in Htc;
+              contradict Htc; easy.
            ++ intros. subst. easy.
            ++ intros. subst. easy.
            ++ intros. subst. easy.
@@ -132,20 +119,15 @@ Proof. intros t Htc.
            ++ intros. subst. easy.
          + destruct IHt as (t', IHt).
            right. cbn.
-           apply term_eqbO_eq in IHt.
            rewrite IHt.
-           case_eq t; try (exists (Fix t'); rewrite term_eqbO_refl; easy).
+           case_eq t; try (exists (Fix t'); easy).
            * intros. rewrite H in IHt. easy.
-       - pose proof Htc as Htc0.
-         specialize (isvalue_dec t1); intros it1.
+       - specialize (isvalue_dec t1); intros it1.
          right.
-         apply istypechecked_plus2 in Htc0.
-         destruct Htc0 as (Ha, Hb).
-         unfold istypechecked in IHt1, IHt2.
-         rewrite Ha in IHt1.
-         rewrite Hb in IHt2.
-         specialize (IHt1 eq_refl).
-         specialize (IHt2 eq_refl).
+         apply istypechecked_plus in Htc.
+         destruct Htc as (Ha, (Hb, Hc)).
+         specialize (IHt1 _ Ha).
+         specialize (IHt2 _ Hb).
          cbn.
          destruct it1 as [it1 | it1].
          + case_eq t1; try (intros; rewrite H in it1; cbn in it1; easy).
@@ -160,15 +142,13 @@ Proof. intros t Htc.
                      case_eq (typecheck (extend nil x tx) e); intros;
                      rewrite H in Hb; contradict Hb; easy.
                    * intros n Ht2 m Ht1.
-                     exists (NVal (m + n)).
-                     rewrite term_eqbO_refl. easy.
+                     exists (NVal (m + n)). easy.
                    * intros b Ht2 n Ht1.
                      rewrite Ht2 in Hb.
                      contradict Hb; easy.
                +++ destruct IHt2 as (t2', Hstep).
-                   apply term_eqbO_eq in Hstep.
                    rewrite Hstep. cbn. intros n Ht1.
-                   case_eq t2; try (exists (Plus (NVal n) t2'); rewrite term_eqbO_refl; easy).
+                   case_eq t2; try (exists (Plus (NVal n) t2'); easy).
                    intros m H1.
                    rewrite H1 in Hstep. cbn in Hstep.
                    contradict Hstep; easy.
@@ -177,21 +157,16 @@ Proof. intros t Htc.
          + destruct IHt1 as [IHt1 | IHt1].
            rewrite it1 in IHt1. easy.
            destruct IHt1 as (t1', Hstep).
-           apply term_eqbO_eq in Hstep.
            rewrite Hstep, it1.
-           case_eq t1; try (exists (Plus t1' t2); rewrite term_eqbO_refl; easy).
+           case_eq t1; try (exists (Plus t1' t2); easy).
            intros n H0.
            subst. easy.
-       - pose proof Htc as Htc0.
-         specialize (isvalue_dec t1); intros it1.
+       - specialize (isvalue_dec t1); intros it1.
          right.
-         apply istypechecked_plus2 in Htc0.
-         destruct Htc0 as (Ha, Hb).
-         unfold istypechecked in IHt1, IHt2.
-         rewrite Ha in IHt1.
-         rewrite Hb in IHt2.
-         specialize (IHt1 eq_refl).
-         specialize (IHt2 eq_refl).
+         apply istypechecked_minus in Htc.
+         destruct Htc as (Ha, (Hb, Hc)).
+         specialize (IHt1 _ Ha).
+         specialize (IHt2 _ Hb).
          cbn.
          destruct it1 as [it1 | it1].
          + case_eq t1; try (intros; rewrite H in it1; cbn in it1; easy).
@@ -206,15 +181,13 @@ Proof. intros t Htc.
                      case_eq (typecheck (extend nil x tx) e); intros;
                      rewrite H in Hb; contradict Hb; easy.
                    * intros n Ht2 m Ht1.
-                     exists (NVal (m - n)).
-                     rewrite term_eqbO_refl. easy.
+                     exists (NVal (m - n)). easy.
                    * intros b Ht2 n Ht1.
                      rewrite Ht2 in Hb.
                      contradict Hb; easy.
                +++ destruct IHt2 as (t2', Hstep).
-                   apply term_eqbO_eq in Hstep.
                    rewrite Hstep. cbn. intros n Ht1.
-                   case_eq t2; try (exists (Minus (NVal n) t2'); rewrite term_eqbO_refl; easy).
+                   case_eq t2; try (exists (Minus (NVal n) t2'); easy).
                    intros m H1.
                    rewrite H1 in Hstep. cbn in Hstep.
                    contradict Hstep; easy.
@@ -223,21 +196,16 @@ Proof. intros t Htc.
          + destruct IHt1 as [IHt1 | IHt1].
            rewrite it1 in IHt1. easy.
            destruct IHt1 as (t1', Hstep).
-           apply term_eqbO_eq in Hstep.
            rewrite Hstep, it1.
-           case_eq t1; try (exists (Minus t1' t2); rewrite term_eqbO_refl; easy).
+           case_eq t1; try (exists (Minus t1' t2); easy).
            intros n H0.
            subst. easy.
-       - pose proof Htc as Htc0.
-         specialize (isvalue_dec t1); intros it1.
+       - specialize (isvalue_dec t1); intros it1.
          right.
-         apply istypechecked_plus2 in Htc0.
-         destruct Htc0 as (Ha, Hb).
-         unfold istypechecked in IHt1, IHt2.
-         rewrite Ha in IHt1.
-         rewrite Hb in IHt2.
-         specialize (IHt1 eq_refl).
-         specialize (IHt2 eq_refl).
+         apply istypechecked_mult in Htc.
+         destruct Htc as (Ha, (Hb, Hc)).
+         specialize (IHt1 _ Ha).
+         specialize (IHt2 _ Hb).
          cbn.
          destruct it1 as [it1 | it1].
          + case_eq t1; try (intros; rewrite H in it1; cbn in it1; easy).
@@ -252,15 +220,13 @@ Proof. intros t Htc.
                      case_eq (typecheck (extend nil x tx) e); intros;
                      rewrite H in Hb; contradict Hb; easy.
                    * intros n Ht2 m Ht1.
-                     exists (NVal (m * n)).
-                     rewrite term_eqbO_refl. easy.
+                     exists (NVal (m * n)). easy.
                    * intros b Ht2 n Ht1.
                      rewrite Ht2 in Hb.
                      contradict Hb; easy.
                +++ destruct IHt2 as (t2', Hstep).
-                   apply term_eqbO_eq in Hstep.
                    rewrite Hstep. cbn. intros n Ht1.
-                   case_eq t2; try (exists (Mult (NVal n) t2'); rewrite term_eqbO_refl; easy).
+                   case_eq t2; try (exists (Mult (NVal n) t2'); easy).
                    intros m H1.
                    rewrite H1 in Hstep. cbn in Hstep.
                    contradict Hstep; easy.
@@ -269,21 +235,17 @@ Proof. intros t Htc.
          + destruct IHt1 as [IHt1 | IHt1].
            rewrite it1 in IHt1. easy.
            destruct IHt1 as (t1', Hstep).
-           apply term_eqbO_eq in Hstep.
            rewrite Hstep, it1.
-           case_eq t1; try (exists (Mult t1' t2); rewrite term_eqbO_refl; easy).
+           case_eq t1; try (exists (Mult t1' t2); easy).
            intros n H0.
            subst. easy.
        - pose proof Htc as Htc0.
          specialize (isvalue_dec t1); intros it1.
          right.
-         apply istypechecked_eq2 in Htc0.
-         destruct Htc0 as (Ha, Hb).
-         unfold istypechecked in IHt1, IHt2.
-         rewrite Ha in IHt1.
-         rewrite Hb in IHt2.
-         specialize (IHt1 eq_refl).
-         specialize (IHt2 eq_refl).
+         apply istypechecked_eq in Htc0.
+         destruct Htc0 as (Ha, (Hb, Hc)).
+         specialize (IHt1 _ Ha).
+         specialize (IHt2 _ Hb).
          cbn.
          destruct it1 as [it1 | it1].
          + case_eq t1; try (intros; rewrite H in it1; cbn in it1; easy).
@@ -298,15 +260,13 @@ Proof. intros t Htc.
                      case_eq (typecheck (extend nil x tx) e); intros;
                      rewrite H in Hb; contradict Hb; easy.
                    * intros n Ht2 m Ht1.
-                     exists (BVal (Nat.eqb m n)).
-                     rewrite term_eqbO_refl. easy.
+                     exists (BVal (Nat.eqb m n)). easy.
                    * intros b Ht2 n Ht1.
                      rewrite Ht2 in Hb.
                      contradict Hb; easy.
                +++ destruct IHt2 as (t2', Hstep).
-                   apply term_eqbO_eq in Hstep.
                    rewrite Hstep. cbn. intros n Ht1.
-                   case_eq t2; try (exists (Eq (NVal n) t2'); rewrite term_eqbO_refl; easy).
+                   case_eq t2; try (exists (Eq (NVal n) t2'); easy).
                    intros m H1.
                    rewrite H1 in Hstep. cbn in Hstep.
                    contradict Hstep; easy.
@@ -315,21 +275,17 @@ Proof. intros t Htc.
          + destruct IHt1 as [IHt1 | IHt1].
            rewrite it1 in IHt1. easy.
            destruct IHt1 as (t1', Hstep).
-           apply term_eqbO_eq in Hstep.
            rewrite Hstep, it1.
-           case_eq t1; try (exists (Eq t1' t2); rewrite term_eqbO_refl; easy).
+           case_eq t1; try (exists (Eq t1' t2); easy).
            intros n H0.
            subst. easy.
        - pose proof Htc as Htc0.
          specialize (isvalue_dec t1); intros it1.
          right.
-         apply istypechecked_eq2 in Htc0.
-         destruct Htc0 as (Ha, Hb).
-         unfold istypechecked in IHt1, IHt2.
-         rewrite Ha in IHt1.
-         rewrite Hb in IHt2.
-         specialize (IHt1 eq_refl).
-         specialize (IHt2 eq_refl).
+         apply istypechecked_gt in Htc0.
+         destruct Htc0 as (Ha, (Hb, Hc)).
+         specialize (IHt1 _ Ha).
+         specialize (IHt2 _ Hb).
          cbn.
          destruct it1 as [it1 | it1].
          + case_eq t1; try (intros; rewrite H in it1; cbn in it1; easy).
@@ -345,17 +301,14 @@ Proof. intros t Htc.
                      rewrite H in Hb; contradict Hb; easy.
                    * intros n Ht2 m Ht1.
                      destruct m.
-                     ** exists (BVal false).
-                        rewrite term_eqbO_refl. easy.
-                     ** exists  (BVal (Nat.leb n m)).
-                        rewrite term_eqbO_refl. easy.
+                     ** exists (BVal false). easy.
+                     ** exists  (BVal (Nat.leb n m)). easy.
                    * intros b Ht2 n Ht1.
                      rewrite Ht2 in Hb.
                      contradict Hb; easy.
                +++ destruct IHt2 as (t2', Hstep).
-                   apply term_eqbO_eq in Hstep.
                    rewrite Hstep. cbn. intros n Ht1.
-                   case_eq t2; try (exists (Gt (NVal n) t2'); rewrite term_eqbO_refl; easy).
+                   case_eq t2; try (exists (Gt (NVal n) t2'); easy).
                    intros m H1.
                    rewrite H1 in Hstep. cbn in Hstep.
                    contradict Hstep; easy.
@@ -364,26 +317,9 @@ Proof. intros t Htc.
          + destruct IHt1 as [IHt1 | IHt1].
            rewrite it1 in IHt1. easy.
            destruct IHt1 as (t1', Hstep).
-           apply term_eqbO_eq in Hstep.
            rewrite Hstep, it1.
-           case_eq t1; try (exists (Gt t1' t2); rewrite term_eqbO_refl; easy).
+           case_eq t1; try (exists (Gt t1' t2); easy).
            intros n H0.
            subst. easy.
 Qed.
 
-
-Lemma progress: forall t T,
-  typecheck nil t  = Some T ->
-  (isvalue t = true) \/ (exists t', beta t = Some t').
-Proof. intros t T Htc.
-       specialize (progressPre t); intros.
-       unfold istypechecked in *.
-       rewrite Htc in H.
-       specialize (H eq_refl).
-       destruct H as [H| H].
-       - now left.
-       - destruct H as (t', Ht').
-         right. exists t'.
-         apply term_eqbO_eq in Ht'. 
-         easy.
-Qed.
